@prefix rdf: <http://www.w3.org/1999/02/22-rdf-syntax-ns#> .
@prefix schema: <http://schema.org/> .
@prefix xsd: <http://www.w3.org/2001/XMLSchema#> .
@prefix rdfs: <http://www.w3.org/2000/01/rdf-schema#> .
@prefix owl: <http://www.w3.org/2002/07/owl#> .
@prefix skos: <http://www.w3.org/2004/02/skos/core#> .
@prefix dcterms: <http://purl.org/dc/terms/> .
@prefix a4g: <http://data.europa.eu/a4g/ontology#> .
@prefix rml: <http://semweb.mmlab.be/ns/rml#> .
@prefix r2rml: <http://www.w3.org/ns/r2rml#> .
@prefix sfrml: <http://data.europa.eu/a4g/mapping/sf-rml/> .
@prefix m8g: <http://data.europa.eu/m8g/> .
@prefix locn: <http://www.w3.org/ns/locn#> .
@prefix shacl: <http://www.w3.org/ns/shacl#> .
@prefix a4g_shape: <http://data.europa.eu/a4g/data-shape#> .
@prefix eli: <http://data.europa.eu/eli/ontology#> .

a4g_shape:cccev-EvidenceType a shacl:NodeShape ;
	rdfs:label "Evidence type" ;
	rdfs:comment "Information about the characteristics of an Evidence. Additional Information: The Evidence Type and the characteristics it describes are not concrete individual responses to a Requirement (i.e. Evidence), but descriptions about the desired form, content, source and/or other characteristics that an actual response should have and provide (e.g. membership of a class of Evidences)." ;
	rdfs:isDefinedBy a4g_shape:acc-shape ;
	shacl:targetClass m8g:EvidenceType .

a4g_shape:acc-shape a owl:Ontology ;
	rdfs:label "eProcurement Ontology Access - core shapes"@en ;
	rdfs:comment "This version is automatically generated from eAccess.xml on 2024-03-15" ;
	dcterms:description "The eProcurement Ontology Access core shapes provides the generic datashape specifications for the eProcurement Ontology Access core."@en ;
	dcterms:title "eProcurement Ontology Access - core shapes"@en ;
	dcterms:created "2021-06-01"^^xsd:date ;
	dcterms:issued "2024-03-15"^^xsd:date ;
	dcterms:license "© European Union, 2014. Unless otherwise noted, the reuse of the Ontology is authorised under the European Union Public Licence v1.2 (https://eupl.eu/)." ;
	dcterms:publisher "http://publications.europa.eu/resource/authority/corporate-body/PUBL" ;
	<http://purl.org/vocab/vann/preferredNamespacePrefix> "epo" ;
	<http://purl.org/vocab/vann/preferredNamespaceUri> "http://data.europa.eu/a4g/ontology#" ;
	rdfs:seeAlso <https://docs.ted.europa.eu/home/index.html>, <https://github.com/OP-TED/ePO/releases>, <https://joinup.ec.europa.eu/collection/eprocurement/solution/eprocurement-ontology/about>, <https://op.europa.eu/en/web/eu-vocabularies/e-procurement> ;
	owl:imports a4g:acc, a4g:acc-restriction, <http://data.europa.eu/eli/ontology#>, <http://data.europa.eu/m8g/>, <http://iflastandards.info/ns/fr/frbr/frbroo/>, <http://purl.org/dc/terms/>, <http://purl.org/vocab/vann/>, <http://www.w3.org/2004/02/skos/core>, <http://www.w3.org/2006/time>, <http://www.w3.org/ns/adms>, <http://www.w3.org/ns/locn>, <http://www.w3.org/ns/org#>, <http://www.w3.org/ns/person>, <http://xmlns.com/foaf/0.1/> ;
	owl:incompatibleWith "3.1.0" ;
	owl:priorVersion "http://data.europa.eu/a4g/data-shape#acc-shape-4.0.2" ;
	owl:versionIRI a4g_shape:acc-shape-4.1.0 ;
	owl:versionInfo "4.1.0" .

m8g:EvidenceType a owl:Class ;
	skos:prefLabel "Evidence type"@en ;
	skos:definition "Information about the characteristics of an Evidence. Additional Information: The Evidence Type and the characteristics it describes are not concrete individual responses to a Requirement (i.e. Evidence), but descriptions about the desired form, content, source and/or other characteristics that an actual response should have and provide (e.g. membership of a class of Evidences)."@en .

dcterms:description a owl:DatatypeProperty ;
	skos:prefLabel "Description"@en ;
	skos:definition "An account of the resource. Additional Information: Description may include but is not limited to: an abstract, a table of contents, a graphical representation, or a free-text account of the resource. WG Approval 30/05/2023 (eli:LegalExpression) An account of the resource. Additional Information: Description may include but is not limited to: an abstract, a table of contents, a graphical representation, or a free-text account of the resource. WG Approval 30/05/2023 (eli:LegalResource)"@en ;
	rdfs:domain [
		rdf:type owl:Class ;
		owl:unionOf (
			m8g:EvidenceTypeList
			eli:LegalExpression
			eli:LegalResource
		) ;
	] ;
	rdfs:range [
		rdf:type owl:Class ;
		owl:unionOf (
			rdf:PlainLiteral
			rdfs:Literal
		) ;
	] .

dcterms:title a owl:ObjectProperty ;
	skos:prefLabel "Title"@en ;
	skos:definition "A name given to the resource. (eli:LegalExpression)"@en ;
	rdfs:domain eli:LegalExpression ;
	rdfs:range rdfs:Literal .

a4g:acc a owl:Ontology ;
	rdfs:label "eProcurement Ontology Access - core"@en ;
	rdfs:comment "This version is automatically generated from eAccess.xml on 2024-03-15" ;
	dcterms:description "The eProcurement Ontology Access core describes the concepts and properties representing the European Public Procurement Access domain. The provision of these semantics offers the basis for a common understanding of the domain for all stakeholders ensuring the quality of data exchange and transparency. The ontology restrictions are published in a separate artefact."@en ;
	dcterms:title "eProcurement Ontology Access - core"@en ;
	dcterms:created "2021-06-01"^^xsd:date ;
	dcterms:issued "2024-03-15"^^xsd:date ;
	dcterms:license "© European Union, 2014. Unless otherwise noted, the reuse of the Ontology is authorised under the European Union Public Licence v1.2 (https://eupl.eu/)." ;
	dcterms:publisher "http://publications.europa.eu/resource/authority/corporate-body/PUBL" ;
	<http://purl.org/vocab/vann/preferredNamespacePrefix> "epo" ;
	<http://purl.org/vocab/vann/preferredNamespaceUri> "http://data.europa.eu/a4g/ontology#" ;
	rdfs:seeAlso <https://docs.ted.europa.eu/home/index.html>, <https://github.com/OP-TED/ePO/releases>, <https://joinup.ec.europa.eu/collection/eprocurement/solution/eprocurement-ontology/about>, <https://op.europa.eu/en/web/eu-vocabularies/e-procurement> ;
	owl:imports <http://data.europa.eu/eli/ontology#>, <http://data.europa.eu/m8g/>, <http://iflastandards.info/ns/fr/frbr/frbroo/>, <http://purl.org/dc/terms/>, <http://purl.org/vocab/vann/>, <http://www.w3.org/2004/02/skos/core>, <http://www.w3.org/2006/time>, <http://www.w3.org/ns/adms>, <http://www.w3.org/ns/locn>, <http://www.w3.org/ns/org#>, <http://www.w3.org/ns/person>, <http://xmlns.com/foaf/0.1/>, a4g:core ;
	owl:incompatibleWith "3.1.0" ;
	owl:priorVersion "http://data.europa.eu/a4g/ontology#acc-4.0.2" ;
	owl:versionIRI a4g:acc-4.1.0 ;
	owl:versionInfo "4.1.0" .

a4g:acc-restriction a owl:Ontology ;
	rdfs:label "eProcurement Ontology Access - core restrictions"@en ;
	rdfs:comment """This version is automatically generated from eAccess.xml on 
                2024-03-15""" ;
	dcterms:description "The eProcurement Ontology Access core restrictions provides the restrictions and the inference-related specifications on the concepts and properties in the eProcurement Ontology Access core."@en ;
	dcterms:title "eProcurement Ontology Access - core restrictions"@en ;
	dcterms:created "2021-06-01"^^xsd:date ;
	dcterms:issued "2024-03-15"^^xsd:date ;
	dcterms:license "© European Union, 2014. Unless otherwise noted, the reuse of the Ontology is authorised under the European Union Public Licence v1.2 (https://eupl.eu/)." ;
	dcterms:publisher "http://publications.europa.eu/resource/authority/corporate-body/PUBL" ;
	<http://purl.org/vocab/vann/preferredNamespacePrefix> "epo" ;
	<http://purl.org/vocab/vann/preferredNamespaceUri> "http://data.europa.eu/a4g/ontology#" ;
	rdfs:seeAlso <https://docs.ted.europa.eu/home/index.html>, <https://github.com/OP-TED/ePO/releases>, <https://joinup.ec.europa.eu/collection/eprocurement/solution/eprocurement-ontology/about>, <https://op.europa.eu/en/web/eu-vocabularies/e-procurement> ;
	owl:imports a4g:acc, <http://data.europa.eu/eli/ontology#>, <http://data.europa.eu/m8g/>, <http://iflastandards.info/ns/fr/frbr/frbroo/>, <http://purl.org/dc/terms/>, <http://purl.org/vocab/vann/>, <http://www.w3.org/2004/02/skos/core>, <http://www.w3.org/2006/time>, <http://www.w3.org/ns/adms>, <http://www.w3.org/ns/locn>, <http://www.w3.org/ns/org#>, <http://www.w3.org/ns/person>, <http://xmlns.com/foaf/0.1/> ;
	owl:incompatibleWith "3.1.0" ;
	owl:priorVersion "http://data.europa.eu/a4g/ontology#acc-restriction-4.0.2" ;
	owl:versionIRI a4g:acc-restriction-4.1.0 ;
	owl:versionInfo "4.1.0" .

a4g_shape:cccev-EvidenceTypeList a shacl:NodeShape ;
	rdfs:label "Evidence type list" ;
	rdfs:comment "Group of Evidence Types for conforming to a Requirement. Additional Information: An Evidence Type List is satisfied, if and only if, for all included Evidence Types in this List, corresponding conformant Evidence(s) are supporting the Requirement having this List. The Evidence Type List describes thus an AND condition on the different Evidence Types within the list and an OR condition between two or more Evidence Type Lists. Combinations of alternative Lists can be provided for a respondent of a Requirement to choose amongst them." ;
	rdfs:isDefinedBy a4g_shape:acc-shape ;
	shacl:targetClass m8g:EvidenceTypeList ;
	shacl:property a4g_shape:cccev-EvidenceTypeList-cccev-specifiesEvidenceType, a4g_shape:cccev-EvidenceTypeList-dct-description, a4g_shape:cccev-EvidenceTypeList-skos-prefLabel .

m8g:EvidenceTypeList a owl:Class ;
	skos:prefLabel "Evidence type list"@en ;
	skos:definition "Group of Evidence Types for conforming to a Requirement. Additional Information: An Evidence Type List is satisfied, if and only if, for all included Evidence Types in this List, corresponding conformant Evidence(s) are supporting the Requirement having this List. The Evidence Type List describes thus an AND condition on the different Evidence Types within the list and an OR condition between two or more Evidence Type Lists. Combinations of alternative Lists can be provided for a respondent of a Requirement to choose amongst them."@en ;
	rdfs:subClassOf [
		rdf:type owl:Restriction ;
		owl:cardinality 1 ;
		owl:onProperty dcterms:description ;
	] .

a4g_shape:cccev-EvidenceTypeList-cccev-specifiesEvidenceType a shacl:PropertyShape ;
	shacl:description "Evidence Type included in this Evidence Type List." ;
	shacl:class m8g:EvidenceType ;
	shacl:name "Specifies evidence type" ;
	shacl:path m8g:specifiesEvidenceType ;
	shacl:sparql [
		shacl:select "SELECT ?this ?that WHERE { ?this <http://data.europa.eu/m8g/specifiesEvidenceType> ?that . ?that <http://data.europa.eu/m8g/specifiesEvidenceType> ?this .}" ;
	] .

a4g_shape:cccev-EvidenceTypeList-dct-description a shacl:PropertyShape ;
	rdfs:isDefinedBy a4g_shape:acc-shape ;
	shacl:name "Description" ;
	shacl:path dcterms:description ;
	shacl:datatype rdf:PlainLiteral ;
	shacl:maxCount 1 ;
	shacl:minCount 1 .

a4g_shape:cccev-EvidenceTypeList-skos-prefLabel a shacl:PropertyShape ;
	rdfs:isDefinedBy a4g_shape:acc-shape ;
	shacl:name "Pref label" ;
	shacl:path skos:prefLabel ;
	shacl:datatype rdf:PlainLiteral .

m8g:specifiesEvidenceType a owl:ObjectProperty ;
	skos:prefLabel "Specifies evidence type"@en ;
	skos:definition "Evidence Type included in this Evidence Type List. (cccev:EvidenceTypeList -> cccev:EvidenceType (+cccev:specifiesEvidenceType))"@en ;
	rdfs:domain m8g:EvidenceTypeList ;
	rdfs:range m8g:EvidenceType .

rdf:PlainLiteral a owl:Class, rdfs:Datatype ;
	skos:prefLabel "Plain literal"@en .

skos:prefLabel a owl:DatatypeProperty ;
	skos:prefLabel "Pref label"@en ;
	rdfs:domain m8g:EvidenceTypeList ;
	rdfs:range rdf:PlainLiteral .

a4g_shape:eli-LegalExpression a shacl:NodeShape ;
	rdfs:label "Legal expression" ;
	rdfs:comment "The intellectual realisation of a legal resource in the form of a \"sequence of signs\" (typically alpha-numeric characters in a legal context). For example, any version of the legal resource whose content is specified and different from others for any reason: language, versions, etc.; Note that ELI ontology accommodates different point of view on what should be considered a new legal resource, or a new legal expression of the same resource. Typically, a consolidated version can be viewed, in the context of ELI, either as separate legal resource (linked to original version and previous consolidated version using corresponding ELI relations), or as a different legal expression of the same legal resource." ;
	rdfs:isDefinedBy a4g_shape:acc-shape ;
	shacl:targetClass eli:LegalExpression ;
	shacl:property a4g_shape:eli-LegalExpression-dct-description, a4g_shape:eli-LegalExpression-dct-identifier, a4g_shape:eli-LegalExpression-dct-title, a4g_shape:eli-LegalExpression-eli-is_realized_by, a4g_shape:eli-LegalExpression-eli-jurisdiction, a4g_shape:eli-LegalExpression-eli-number .

eli:LegalExpression a owl:Class ;
	skos:prefLabel "Legal expression"@en ;
	skos:definition "The intellectual realisation of a legal resource in the form of a \"sequence of signs\" (typically alpha-numeric characters in a legal context). For example, any version of the legal resource whose content is specified and different from others for any reason: language, versions, etc.; Note that ELI ontology accommodates different point of view on what should be considered a new legal resource, or a new legal expression of the same resource. Typically, a consolidated version can be viewed, in the context of ELI, either as separate legal resource (linked to original version and previous consolidated version using corresponding ELI relations), or as a different legal expression of the same legal resource."@en ;
	rdfs:subClassOf [
		rdf:type owl:Restriction ;
		owl:cardinality 1 ;
		owl:onProperty eli:is_realized_by ;
	], [
		rdf:type owl:Restriction ;
		owl:onProperty dcterms:title ;
		owl:minCardinality 1 ;
	] .

a4g_shape:eli-LegalExpression-dct-description a shacl:PropertyShape ;
	rdfs:isDefinedBy a4g_shape:acc-shape ;
	shacl:description "An account of the resource. Additional Information: Description may include but is not limited to: an abstract, a table of contents, a graphical representation, or a free-text account of the resource. WG Approval 30/05/2023" ;
	shacl:name "Description" ;
	shacl:path dcterms:description .

a4g_shape:eli-LegalExpression-dct-identifier a shacl:PropertyShape ;
	rdfs:isDefinedBy a4g_shape:acc-shape ;
	shacl:description "An unambiguous reference to the resource within a given context." ;
	shacl:name "Identifier" ;
	shacl:path dcterms:identifier ;
	shacl:datatype xsd:anyURI .

a4g_shape:eli-LegalExpression-dct-title a shacl:PropertyShape ;
	rdfs:isDefinedBy a4g_shape:acc-shape ;
	shacl:description "A name given to the resource." ;
	shacl:name "Title" ;
	shacl:path dcterms:title ;
	shacl:minCount 1 .

a4g_shape:eli-LegalExpression-eli-is_realized_by a shacl:PropertyShape ;
	shacl:description "Relates a work to an expression of this work in the form of a \"sequence of signs\" (typically alpha-numeric characters in a legal context). Inverse of \"realizes\"." ;
	shacl:class eli:Work ;
	shacl:name "Is_realized_by" ;
	shacl:path eli:is_realized_by ;
	shacl:sparql [
		shacl:select "SELECT ?this ?that WHERE { ?this <http://data.europa.eu/eli/ontology#is_realized_by> ?that . ?that <http://data.europa.eu/eli/ontology#is_realized_by> ?this .}" ;
	] ;
	shacl:maxCount 1 ;
	shacl:minCount 1 .

a4g_shape:eli-LegalExpression-eli-jurisdiction a shacl:PropertyShape ;
	shacl:description "The jurisdiction from which the legal resource originates. The place identifier can be taken from the Administrative Territorial Unit table published of the EU Publications Office at https://op.europa.eu/en/web/eu-vocabularies/at-dataset/-/resource/dataset/atu. Member States don't have to recreate their own list of values." ;
	shacl:class <http://publications.europa.eu/resource/authority/atu> ;
	shacl:name "Jurisdiction" ;
	shacl:path eli:jurisdiction .

a4g_shape:eli-LegalExpression-eli-number a shacl:PropertyShape ;
	rdfs:isDefinedBy a4g_shape:acc-shape ;
	shacl:description "An identifier or other disambiguating feature for a legal resource or legal expression. This can be the number of a legislation, the number of an article, or the issue number of an official journal." ;
	shacl:name "Number" ;
	shacl:path eli:number ;
	shacl:datatype xsd:string .

dcterms:identifier a owl:DatatypeProperty ;
	skos:prefLabel "Identifier"@en ;
	skos:definition "An unambiguous reference to the resource within a given context. (eli:LegalExpression) An unambiguous reference to the resource within a given context. (eli:LegalResource)"@en ;
	rdfs:domain [
		rdf:type owl:Class ;
		owl:unionOf (
			eli:LegalExpression
			eli:LegalResource
		) ;
	] ;
	rdfs:range xsd:anyURI .

xsd:anyURI a rdfs:Datatype ;
	skos:prefLabel "Any u r i"@en .

eli:Work a owl:Class ;
	skos:prefLabel "Work"@en ;
	skos:definition "Any distinct intellectual creation (i.e., the intellectual content), in the context of ELI. The substance of Work is ideas."@en .

eli:is_realized_by a owl:ObjectProperty, owl:FunctionalProperty ;
	skos:prefLabel "Is_realized_by"@en ;
	skos:definition "Relates a work to an expression of this work in the form of a \"sequence of signs\" (typically alpha-numeric characters in a legal context). Inverse of \"realizes\". (eli:LegalExpression -> eli:Work (+eli:is_realized_by))"@en ;
	rdfs:domain eli:LegalExpression ;
	rdfs:range eli:Work .

eli:jurisdiction a owl:ObjectProperty ;
	skos:prefLabel "Jurisdiction"@en ;
	skos:definition "The jurisdiction from which the legal resource originates. The place identifier can be taken from the Administrative Territorial Unit table published of the EU Publications Office at https://op.europa.eu/en/web/eu-vocabularies/at-dataset/-/resource/dataset/atu. Member States don't have to recreate their own list of values. (eli:LegalExpression -> at-voc:atu (+eli:jurisdiction)) The jurisdiction from which the legal resource originates. The place identifier can be taken from the Administrative Territorial Unit table published of the EU Publications Office at https://op.europa.eu/en/web/eu-vocabularies/at-dataset/-/resource/dataset/atu. Member States don't have to recreate their own list of values. (eli:LegalResource -> at-voc:atu (+eli:jurisdiction))"@en ;
	rdfs:domain [
		rdf:type owl:Class ;
		owl:unionOf (
			eli:LegalExpression
			eli:LegalResource
		) ;
	] ;
	rdfs:range skos:Concept .

eli:number a owl:DatatypeProperty ;
	skos:prefLabel "Number"@en ;
	skos:definition "An identifier or other disambiguating feature for a legal resource or legal expression. This can be the number of a legislation, the number of an article, or the issue number of an official journal. (eli:LegalExpression) An identifier or other disambiguating feature for a legal resource or legal expression. This can be the number of a legislation, the number of an article, or the issue number of an official journal. (eli:LegalResource)"@en ;
	rdfs:domain [
		rdf:type owl:Class ;
		owl:unionOf (
			eli:LegalExpression
			eli:LegalResource
		) ;
	] ;
	rdfs:range xsd:string .

a4g_shape:eli-LegalResource a shacl:NodeShape ;
	rdfs:label "Legal resource" ;
	rdfs:comment "A work in a legislative corpus. This applies to acts that have been legally enacted (whether or not they are still in force). For example, the abstract concept of the legal resource; e.g. \"act 3 of 2005\" (adapted from Akoma Ntoso) A legal resource can represent a legal act or any component of a legal act, like an article. Legal resources can be linked together using properties defined in the model. Note that ELI ontology accommodates different point of view on what should be considered a new legal resource, or a new legal expression of the same resource. Typically, a consolidated version can be viewed, in the context of ELI, either as separate legal resource (linked to original version and previous consolidated version using corresponding ELI relations), or as a different legal expression of the same legal resource." ;
	rdfs:isDefinedBy a4g_shape:acc-shape ;
	shacl:targetClass eli:LegalResource ;
	shacl:property a4g_shape:eli-LegalResource-dct-description, a4g_shape:eli-LegalResource-dct-identifier, a4g_shape:eli-LegalResource-eli-jurisdiction, a4g_shape:eli-LegalResource-eli-number, a4g_shape:eli-LegalResource-epo-hasResourceType .

eli:LegalResource a owl:Class ;
	skos:prefLabel "Legal resource"@en ;
	skos:definition "A work in a legislative corpus. This applies to acts that have been legally enacted (whether or not they are still in force). For example, the abstract concept of the legal resource; e.g. \"act 3 of 2005\" (adapted from Akoma Ntoso) A legal resource can represent a legal act or any component of a legal act, like an article. Legal resources can be linked together using properties defined in the model. Note that ELI ontology accommodates different point of view on what should be considered a new legal resource, or a new legal expression of the same resource. Typically, a consolidated version can be viewed, in the context of ELI, either as separate legal resource (linked to original version and previous consolidated version using corresponding ELI relations), or as a different legal expression of the same legal resource."@en ;
	rdfs:subClassOf eli:Work, [
		rdf:type owl:Restriction ;
		owl:cardinality 1 ;
		owl:onProperty dcterms:description ;
	] .

a4g_shape:eli-LegalResource-dct-description a shacl:PropertyShape ;
	rdfs:isDefinedBy a4g_shape:acc-shape ;
	shacl:description "An account of the resource. Additional Information: Description may include but is not limited to: an abstract, a table of contents, a graphical representation, or a free-text account of the resource. WG Approval 30/05/2023" ;
	shacl:name "Description" ;
	shacl:path dcterms:description ;
	shacl:maxCount 1 ;
	shacl:minCount 1 .

a4g_shape:eli-LegalResource-dct-identifier a shacl:PropertyShape ;
	rdfs:isDefinedBy a4g_shape:acc-shape ;
	shacl:description "An unambiguous reference to the resource within a given context." ;
	shacl:name "Identifier" ;
	shacl:path dcterms:identifier ;
	shacl:datatype xsd:anyURI .

a4g_shape:eli-LegalResource-eli-jurisdiction a shacl:PropertyShape ;
	shacl:description "The jurisdiction from which the legal resource originates. The place identifier can be taken from the Administrative Territorial Unit table published of the EU Publications Office at https://op.europa.eu/en/web/eu-vocabularies/at-dataset/-/resource/dataset/atu. Member States don't have to recreate their own list of values." ;
	shacl:class <http://publications.europa.eu/resource/authority/atu> ;
	shacl:name "Jurisdiction" ;
	shacl:path eli:jurisdiction .

a4g_shape:eli-LegalResource-eli-number a shacl:PropertyShape ;
	rdfs:isDefinedBy a4g_shape:acc-shape ;
	shacl:description "An identifier or other disambiguating feature for a legal resource or legal expression. This can be the number of a legislation, the number of an article, or the issue number of an official journal." ;
	shacl:name "Number" ;
	shacl:path eli:number ;
	shacl:datatype xsd:string .

a4g_shape:eli-LegalResource-epo-hasResourceType a shacl:PropertyShape ;
	shacl:class <http://publications.europa.eu/resource/authority/resource-type> ;
	shacl:name "Has resource type" ;
	shacl:path a4g:hasResourceType ;
	shacl:minCount 1 .

a4g:hasResourceType a owl:ObjectProperty ;
	rdfs:isDefinedBy a4g:acc ;
	skos:prefLabel "Has resource type"@en ;
	rdfs:domain eli:LegalResource ;
	rdfs:range skos:Concept .

a4g_shape:eli-LegalResourceSubdivision a shacl:NodeShape ;
	rdfs:label "Legal resource subdivision" ;
	rdfs:comment "A component of a legal act, at an arbitrary level of precision, like a chapter, an article, an alinea, a paragraph or an list item." ;
	rdfs:isDefinedBy a4g_shape:acc-shape ;
	shacl:targetClass eli:LegalResourceSubdivision ;
	shacl:property a4g_shape:eli-LegalResourceSubdivision-epo-hasSubdivision .

eli:LegalResourceSubdivision a owl:Class ;
	skos:prefLabel "Legal resource subdivision"@en ;
	skos:definition "A component of a legal act, at an arbitrary level of precision, like a chapter, an article, an alinea, a paragraph or an list item."@en ;
	rdfs:subClassOf eli:LegalResource .

a4g_shape:eli-LegalResourceSubdivision-epo-hasSubdivision a shacl:PropertyShape ;
	shacl:class <http://publications.europa.eu/resource/authority/subdivision> ;
	shacl:name "Has subdivision" ;
	shacl:path a4g:hasSubdivision ;
	shacl:maxCount 1 .

a4g:hasSubdivision a owl:ObjectProperty ;
	rdfs:isDefinedBy a4g:acc ;
	skos:prefLabel "Has subdivision"@en ;
	rdfs:domain eli:LegalResourceSubdivision ;
	rdfs:range skos:Concept .

a4g_shape:eli-Work a shacl:NodeShape ;
	rdfs:label "Work" ;
	rdfs:comment "Any distinct intellectual creation (i.e., the intellectual content), in the context of ELI. The substance of Work is ideas." ;
	rdfs:isDefinedBy a4g_shape:acc-shape ;
	shacl:targetClass eli:Work ;
	shacl:property a4g_shape:eli-Work-dct-isPartOf .

a4g_shape:eli-Work-dct-isPartOf a shacl:PropertyShape ;
	shacl:description "A related resource in which the described resource is physically or logically included." ;
	shacl:class eli:Work ;
	shacl:name "Is part of" ;
	shacl:path dcterms:isPartOf ;
	shacl:sparql [
		shacl:select "SELECT ?this ?that WHERE { ?this <http://purl.org/dc/terms/isPartOf> ?that . ?that <http://purl.org/dc/terms/isPartOf> ?this .}" ;
	] .

dcterms:isPartOf a owl:ObjectProperty, owl:AsymmetricProperty ;
	skos:prefLabel "Is part of"@en ;
	skos:definition "A related resource in which the described resource is physically or logically included. (eli:Work -> eli:Work (+dct:isPartOf))"@en ;
	rdfs:domain eli:Work ;
	rdfs:range eli:Work .

a4g_shape:epo-acc-ESPDRequest a shacl:NodeShape ;
	rdfs:label "E s p d request" ;
	rdfs:comment "An updated self-declaration used by the economic operator as a preliminary evidence in replacement of certificates issued by public authorities or third parties confirming that the economic operator fulfils the Exclusion Grounds and the Selection Criteria set out by the Buyer for a specific Procurement. WG Approval 05/03/2024" ;
	rdfs:isDefinedBy a4g_shape:acc-shape ;
	shacl:targetClass a4g:ESPDRequest .

a4g:ESPDRequest a owl:Class ;
	rdfs:isDefinedBy a4g:acc ;
	skos:prefLabel "E s p d request"@en ;
	skos:definition "An updated self-declaration used by the economic operator as a preliminary evidence in replacement of certificates issued by public authorities or third parties confirming that the economic operator fulfils the Exclusion Grounds and the Selection Criteria set out by the Buyer for a specific Procurement. WG Approval 05/03/2024"@en ;
	rdfs:subClassOf a4g:Document .

a4g_shape:epo-acc-ESPDRequest-epo-concernsProcedure shacl:description "The relations epo-acc:concernsProcedure and epo:refersToProcedure have to refer to the same Procedure." .

a4g:concernsProcedure a owl:ObjectProperty ;
	rdfs:isDefinedBy a4g:acc ;
	skos:prefLabel "Concerns procedure"@en ;
	skos:definition "Relates to Procedure. WG approval 05/03/2024 (epo-acc:ESPDRequest -> epo:Procedure (+epo:concernsProcedure))"@en ;
	skos:editorialNote "The relations epo-acc:concernsProcedure and epo:refersToProcedure have to refer to the same Procedure."@en ;
	rdfs:domain a4g:ESPDRequest ;
	rdfs:range a4g:Procedure .

a4g:refersToNotice a owl:ObjectProperty ;
	rdfs:isDefinedBy a4g:acc ;
	skos:prefLabel "Refers to notice"@en ;
	skos:definition "Reference to a Notice. WG approval 12/03/2024 (epo-acc:ESPDRequest -> epo:Notice (+epo-acc:refersToNotice))"@en ;
	rdfs:domain a4g:ESPDRequest ;
	rdfs:range a4g:Notice .

a4g:specifiesProcurementCriterion a owl:ObjectProperty ;
	rdfs:isDefinedBy a4g:acc ;
	skos:prefLabel "Specifies procurement criterion"@en ;
	rdfs:domain a4g:ESPDRequest ;
	rdfs:range a4g:ProcurementCriterion .

eli:uri_schema a owl:ObjectProperty ;
	skos:prefLabel "Uri_schema"@en ;
	skos:definition "Schema describing the URI of an ELI instance. ELI uses URI template specifications (IETF RFC 6570). Schemes should be associated with member states and will be published in a registry. (eli:LegalExpression -> adms:Identifier (+eli:uri_schema)) Schema describing the URI of an ELI instance. ELI uses URI template specifications (IETF RFC 6570). Schemes should be associated with member states and will be published in a registry. (eli:LegalResourceSubdivision -> adms:Identifier (+eli:uri_schema))"@en ;
	rdfs:domain [
		rdf:type owl:Class ;
		owl:unionOf (
			eli:LegalExpression
			eli:LegalResourceSubdivision
		) ;
	] ;
	rdfs:range <http://www.w3.org/ns/adms#Identifier> .

m8g:hasEvidenceTypeList a owl:ObjectProperty ;
	skos:prefLabel "Has evidence type list"@en ;
	skos:definition "Evidence Type List that specifies the Evidence Types that are needed to meet the Requirement. Additional Information: One or several Lists of Evidence Types can support a Requirement. At least one of them must be satisfied by the response to the Requirement. (cccev:InformationRequirement -> cccev:EvidenceTypeList (+cccev:hasEvidenceTypeList))"@en ;
	rdfs:domain m8g:InformationRequirement ;
	rdfs:range m8g:EvidenceTypeList .

m8g:isDerivedFrom a owl:ObjectProperty ;
	skos:prefLabel "Is derived from"@en ;
	skos:definition "Reference Framework on which the Requirement is based, such as a law or regulation. Additional Information: The relation between a parent Requirement and a sub-Requirement can be complex. Therefore, qualified relations (see hasQualifiedRelation) can be used to represent this relationship on its own and qualify it with additional information such as a date, a place. This is left to implementers. In the case where the purpose is to link the two Requirements without additional information, the simple relationship as proposed here can be directly used. (cccev:Requirement -> eli:LegalResource (+cccev:isDerivedFrom))"@en ;
	rdfs:domain m8g:Requirement ;
	rdfs:range eli:LegalResource .

m8g:validityPeriodConstraint a owl:ObjectProperty ;
	skos:prefLabel "Validity period constraint"@en ;
	skos:definition "Temporal condition on the validity period of the Evidence Type. Additional Information: E.g. A Belgian birth evidence is valid for X months after emission. To express constraints on the validity period that must hold when assessing the evidence (e.g. the certificate of good conduct cannot be issued more than 3 months ago), we refer to the Constraint class. (cccev:EvidenceType -> epo:Period (+cccev:validityPeriodConstraint))"@en ;
	rdfs:domain m8g:EvidenceType ;
	rdfs:range a4g:Period .

dcterms:conformsTo a owl:ObjectProperty ;
	skos:prefLabel "Conforms to"@en ;
	skos:definition "An established standard to which the described resource conforms. Additional Information: Examples of characteristics could be the layout or the configuration of the Evidence. (cccev:Evidence -> cccev:EvidenceType (+dct:conformsTo))"@en ;
	rdfs:domain m8g:Evidence ;
	rdfs:range m8g:EvidenceType .

dcterms:language a owl:ObjectProperty ;
	skos:prefLabel "Language"@en ;
	skos:definition "A language of the resource. (eli:LegalExpression -> at-voc:language (+dct:language))"@en ;
	rdfs:domain eli:LegalExpression ;
	rdfs:range skos:Concept .

xsd:boolean a rdfs:Datatype ;
	skos:prefLabel "Boolean"@en .

xsd:date a rdfs:Datatype ;
	skos:prefLabel "Date"@en .

xsd:dateTime a rdfs:Datatype ;
	skos:prefLabel "Date time"@en .

xsd:decimal a rdfs:Datatype ;
	skos:prefLabel "Decimal"@en .

xsd:integer a rdfs:Datatype ;
	skos:prefLabel "Integer"@en .

<http://www.w3.org/ns/adms#identifier> a owl:ObjectProperty ;
	skos:prefLabel "Identifier"@en ;
	skos:definition "Links a resource to an adms:Identifier class. (cccev:EvidenceType -> adms:Identifier (+adms:identifier)) Links a resource to an adms:Identifier class. (cccev:EvidenceTypeList -> adms:Identifier (+adms:identifier))"@en ;
	rdfs:domain [
		rdf:type owl:Class ;
		owl:unionOf (
			m8g:EvidenceType
			m8g:EvidenceTypeList
		) ;
	] ;
	rdfs:range <http://www.w3.org/ns/adms#Identifier> .

rdfs:Literal a owl:Class .

