@prefix rdf: <http://www.w3.org/1999/02/22-rdf-syntax-ns#> .
@prefix schema: <http://schema.org/> .
@prefix xsd: <http://www.w3.org/2001/XMLSchema#> .
@prefix rdfs: <http://www.w3.org/2000/01/rdf-schema#> .
@prefix owl: <http://www.w3.org/2002/07/owl#> .
@prefix skos: <http://www.w3.org/2004/02/skos/core#> .
@prefix dcterms: <http://purl.org/dc/terms/> .
@prefix : <http://data.europa.eu/a4g/ontology#> .
@prefix sh: <http://www.w3.org/ns/shacl#> .
@prefix a4g_shape: <http://data.europa.eu/a4g/data-shape#> .

:ESPDRequest a owl:Class ;
	rdfs:isDefinedBy :acc ;
	skos:prefLabel "ESPD request"@en ;
	rdfs:subClassOf :Document ;
	skos:definition "An updated self-declaration used by the economic operator as a preliminary evidence in replacement of certificates issued by public authorities or third parties confirming that the economic operator fulfils the Exclusion Grounds and the Selection Criteria set out by the Buyer for a specific Procurement. WG Approval 05/03/2024"@en .

:concernsProcedure a owl:ObjectProperty ;
	rdfs:isDefinedBy :acc ;
	skos:prefLabel "Concerns procedure"@en ;
	rdfs:domain :ESPDRequest ;
	rdfs:range :Procedure ;
	skos:definition "Relates to Procedure. WG approval 05/03/2024 (epo-acc:ESPDRequest -> epo:Procedure (+epo:concernsProcedure))"@en ;
	skos:editorialNote "The relations epo-acc:concernsProcedure and epo:refersToProcedure have to refer to the same Procedure."@en .

:refersToNotice a owl:ObjectProperty ;
	rdfs:isDefinedBy :acc ;
	skos:prefLabel "Refers to notice"@en ;
	rdfs:domain :ESPDRequest ;
	rdfs:range :Notice ;
	skos:definition "Reference to a Notice. WG approval 12/03/2024 (epo-acc:ESPDRequest -> epo:Notice (+epo-acc:refersToNotice))"@en .

:specifiesProcurementCriterion a owl:ObjectProperty ;
	rdfs:isDefinedBy :acc ;
	skos:prefLabel "Specifies procurement criterion"@en ;
	rdfs:domain :ESPDRequest ;
	rdfs:range :ProcurementCriterion .

## Shapes

a4g_shape:ESPDRequestShape
  a sh:NodeShape ;
  rdfs:isDefinedBy a4g_shape:acc-shape ;
  sh:targetClass :ESPDRequest ;
  sh:property [
    sh:path :concernsProcedure ;
    sh:minCount 1 ;
    sh:maxCount 1 ;
    sh:nodeKind sh:IRI ;
    sh:class :Procedure ;
  ] ;
  sh:property [
    sh:path :refersToNotice ;
    sh:minCount 0 ;
    sh:nodeKind sh:IRI ;
    sh:class :Notice ;
  ] ;
  sh:property [
    sh:path :specifiesProcurementCriterion ;
    sh:minCount 1 ;
    sh:nodeKind sh:IRI ;
    sh:class :ProcurementCriterion ;
  ] .

## Metadata

:acc a owl:Ontology ;
	rdfs:label "eProcurement Ontology Access - core"@en ;
	rdfs:comment "This version is automatically generated from eAccess.xml on 2024-03-15" ;
	dcterms:description "The eProcurement Ontology Access core describes the concepts and properties representing the European Public Procurement Access domain. The provision of these semantics offers the basis for a common understanding of the domain for all stakeholders ensuring the quality of data exchange and transparency. The ontology restrictions are published in a separate artefact."@en ;
	dcterms:title "eProcurement Ontology Access - core"@en ;
	dcterms:created "2021-06-01"^^xsd:date ;
	dcterms:issued "2024-03-15"^^xsd:date ;
	dcterms:license "© European Union, 2014. Unless otherwise noted, the reuse of the Ontology is authorised under the European Union Public Licence v1.2 (https://eupl.eu/)." ;
	dcterms:publisher "http://publications.europa.eu/resource/authority/corporate-body/PUBL" ;
	<http://purl.org/vocab/vann/preferredNamespacePrefix> "epo" ;
	<http://purl.org/vocab/vann/preferredNamespaceUri> "http://data.europa.eu/a4g/ontology#" ;
	rdfs:seeAlso <https://docs.ted.europa.eu/home/index.html>, <https://github.com/OP-TED/ePO/releases>, <https://joinup.ec.europa.eu/collection/eprocurement/solution/eprocurement-ontology/about>, <https://op.europa.eu/en/web/eu-vocabularies/e-procurement> ;
	owl:imports <http://data.europa.eu/eli/ontology#>, <http://data.europa.eu/m8g/>, <http://iflastandards.info/ns/fr/frbr/frbroo/>, <http://purl.org/dc/terms/>, <http://purl.org/vocab/vann/>, <http://www.w3.org/2004/02/skos/core>, <http://www.w3.org/2006/time>, <http://www.w3.org/ns/adms>, <http://www.w3.org/ns/locn>, <http://www.w3.org/ns/org#>, <http://www.w3.org/ns/person>, <http://xmlns.com/foaf/0.1/>, :core ;
	owl:incompatibleWith "3.1.0" ;
	owl:priorVersion :acc-4.0.2 ;
	owl:versionIRI :acc-4.1.0 ;
	owl:versionInfo "4.1.0" .

a4g_shape:acc-shape a owl:Ontology ;
	rdfs:label "eProcurement Ontology Access - core shapes"@en ;
	rdfs:comment "This version is automatically generated from eAccess.xml on 2024-03-15" ;
	dcterms:description "The eProcurement Ontology Access core shapes provides the generic datashape specifications for the eProcurement Ontology Access core."@en ;
	dcterms:title "eProcurement Ontology Access - core shapes"@en ;
	dcterms:created "2021-06-01"^^xsd:date ;
	dcterms:issued "2024-03-15"^^xsd:date ;
	dcterms:license "© European Union, 2014. Unless otherwise noted, the reuse of the Ontology is authorised under the European Union Public Licence v1.2 (https://eupl.eu/)." ;
	dcterms:publisher "http://publications.europa.eu/resource/authority/corporate-body/PUBL" ;
	rdfs:seeAlso <https://docs.ted.europa.eu/home/index.html>, <https://github.com/OP-TED/ePO/releases>, <https://joinup.ec.europa.eu/collection/eprocurement/solution/eprocurement-ontology/about>, <https://op.europa.eu/en/web/eu-vocabularies/e-procurement> ;
	owl:imports :acc, :acc-restriction, <http://data.europa.eu/eli/ontology#>, <http://data.europa.eu/m8g/>, <http://iflastandards.info/ns/fr/frbr/frbroo/>, <http://purl.org/dc/terms/>, <http://purl.org/vocab/vann/>, <http://www.w3.org/2004/02/skos/core>, <http://www.w3.org/2006/time>, <http://www.w3.org/ns/adms>, <http://www.w3.org/ns/locn>, <http://www.w3.org/ns/org#>, <http://www.w3.org/ns/person>, <http://xmlns.com/foaf/0.1/> ;
    owl:versionInfo "4.1.0" ;
	owl:incompatibleWith "3.1.0" ;
	owl:priorVersion a4g_shape:acc-shape-4.0.2 ;
	owl:versionIRI a4g_shape:acc-shape-4.1.0 .

